update file for proof
- proof of 10.4.5
- proofs of unification and productiveness
- admitted helper lemmas

B_Unification/lowenheim_proof.v
@@ -14,217 +14,24 @@ Require Export lowenheim_formula.
 Require Import List.
 Import ListNotations.
 
+(*** 3. Lownheim's proof ***)
 
+(* In this subsection we provide a proof that our lownheim substituion builder produces a substituion
+   that 
+      -> unifies any given term (if possible)
+      -> is a reproductive unifier, hence an mgu *)
 
 
 (** 3.1 Declarations useful for the proof **)
-
-
-Axiom refl_comm :
-  forall t1 t2, t1 == t2 -> t2 == t1.
-
-Lemma subst_distr_opp :
-  forall s x y, apply_subst (x + y) s == apply_subst x s + apply_subst y s.
-Proof.
-  intros.
-  apply refl_comm.
-  apply subst_distribution.
-Qed. 
-
-
-Lemma subst_mul_distr_opp :
-  forall s x y, apply_subst (x * y) s == apply_subst x s * apply_subst y s.
-Proof.
-  intros.
-  apply refl_comm.
-  apply subst_associative.
-Qed. 
-
-
-Lemma sum_assoc_opp :
- forall x y z, x + (y + z) == (x + y) + z.
-Proof.
-Admitted.
-
-Lemma mul_assoc_opp :
- forall x y z, x * (y * z) == (x * y) * z.
-Proof.
-Admitted.
-
-
-
-Lemma var_subst:
-  forall (v : var) (ts : term) ,
-  (apply_subst (VAR v) (cons (v , ts) nil) ) == ts.
-Proof.
-Admitted.
-
-
-
-
 
 
 Definition sub_term (t : term) (t' : term) : Prop :=
   forall (x : var ),
   (In x (term_unique_vars t) ) -> (In x (term_unique_vars t')) .
 
-Lemma sub_term_v :
-  forall (v : var),
-  sub_term (VAR v) (VAR v).
- Proof.
-Admitted.
 
-Fixpoint build_on_list_of_vars (list_var : var_set) (s : term) (sig1 : subst) (sig2 : subst) : subst :=
-  match list_var with 
-   | nil => nil 
-   | v' :: v =>
-      (cons (v' , (s + T1) * (apply_subst (VAR v') sig1 )  + s * (apply_subst (VAR v' ) sig2 )  )    
-            (build_on_list_of_vars v s sig1 sig2) )
-  end. 
+(** 3.2 Lemmas useful for the proof  **)
 
-
-Lemma helper_1:
-forall (t' s : term) (v : var) (sig1 sig2 : subst),
-  sub_term (VAR v) t' -> 
-  apply_subst (VAR v) (build_on_list_of_vars (term_unique_vars t') s sig1 sig2)
-  == 
-  apply_subst (VAR v) (build_on_list_of_vars (term_unique_vars (VAR v)) s sig1 sig2).
-Proof.
-Admitted.
-
-Lemma helper_2a:
-  forall (t1 t2 t' : term),
-  sub_term (t1 + t2) t' -> sub_term t1 t'.
-Proof.
-Admitted. 
-  
-Lemma helper_2b:
-  forall (t1 t2 t' : term),
-  sub_term (t1 + t2) t' -> sub_term t2 t'.
-Proof.
-Admitted. 
-
-
-
-
-
-(* Lemma 10.4.3*)
-
-Lemma subs_distr_vars_ver2 :
-  forall (t t' : term) (s : term) (sig1 sig2 : subst) (l : list var),
-  (sub_term t t') ->
-  apply_subst t (build_on_list_of_vars  (term_unique_vars t') s sig1 sig2)
-    ==
-  (s + T1) * (apply_subst t sig1) + s * (apply_subst t sig2).
-Proof.
- intros. generalize dependent t'.  induction t.
-  - intros t'. repeat rewrite ground_term_cannot_subst.
-    + rewrite mul_comm with (x := s + T1). rewrite distr. repeat rewrite mul_T0_x. rewrite mul_comm with (x := s).
-      rewrite mul_T0_x.  repeat rewrite sum_x_x. reflexivity.
-    + unfold ground_term. reflexivity.
-    + unfold ground_term. reflexivity.
-    + unfold ground_term. reflexivity.
-  - intros t'. repeat rewrite ground_term_cannot_subst.
-    + rewrite mul_comm with (x := s + T1). rewrite mul_id. rewrite mul_comm with (x := s). rewrite mul_id. rewrite sum_comm with (x := s).
-      repeat rewrite sum_assoc. rewrite sum_x_x.  rewrite sum_comm with (x := T1). rewrite sum_id. reflexivity.
-    +  unfold ground_term. reflexivity.
-    +  unfold ground_term. reflexivity.
-    + unfold ground_term. reflexivity.
-  - intros. rewrite helper_1 .
-    + unfold term_unique_vars. unfold term_vars. unfold var_set_create_unique. unfold var_set_includes_var. unfold build_on_list_of_vars.
-    rewrite var_subst. reflexivity. 
-    + apply H. 
-  -  intros. specialize (IHt1 t'). specialize (IHt2 t').  repeat rewrite subst_distr_opp. 
-      rewrite IHt1. rewrite IHt2.
-    + rewrite distr. rewrite distr. repeat rewrite sum_assoc. rewrite sum_comm with (x := (s + T1) * apply_subst t2 sig1)
-      (y := (s * apply_subst t1 sig2 + s * apply_subst t2 sig2)). repeat rewrite sum_assoc.
-      rewrite sum_comm with (x := s * apply_subst t2 sig2 ) (y := (s + T1) * apply_subst t2 sig1).
-      repeat rewrite sum_assoc. reflexivity.
-    + pose helper_2b as H2. specialize (H2 t1 t2 t'). apply H2. apply H. 
-    + pose helper_2a as H2. specialize (H2 t1 t2 t'). apply H2. apply H. 
-  - intros. specialize (IHt1 t'). specialize (IHt2 t'). repeat rewrite subst_mul_distr_opp. rewrite IHt1. rewrite IHt2.
-    + rewrite distr. rewrite mul_comm with (y := ((s + T1) * apply_subst t2 sig1)).
-    rewrite distr. rewrite mul_comm with (y := (s * apply_subst t2 sig2)). rewrite distr.
-    repeat rewrite mul_assoc. repeat rewrite mul_comm with (x := apply_subst t2 sig1).
-    repeat rewrite mul_assoc.
-    rewrite mul_assoc_opp with (x := (s + T1)) (y := (s + T1)) . rewrite mul_x_x.
-    rewrite mul_assoc_opp with (x := (s + T1)) (y := s). rewrite mul_comm with (x := (s + T1)) (y := s).
-    rewrite distr. rewrite mul_x_x. rewrite mul_id_sym. rewrite sum_x_x. rewrite mul_T0_x.
-    repeat rewrite mul_assoc. rewrite mul_comm with (x := apply_subst t2 sig2 ).
-    repeat rewrite mul_assoc. rewrite mul_assoc_opp with (x := s ) (y := (s + T1)).
-    rewrite distr. rewrite mul_x_x. rewrite mul_id_sym. rewrite sum_x_x. rewrite mul_T0_x.
-    repeat rewrite sum_assoc. rewrite sum_assoc_opp with (x := T0) (y := T0). rewrite sum_x_x. rewrite sum_id.
-    repeat rewrite mul_assoc. rewrite mul_comm with (x := apply_subst t2 sig2) (y := s * apply_subst t1 sig2).
-    repeat rewrite mul_assoc. rewrite mul_assoc_opp with (x := s). rewrite mul_x_x. reflexivity.
-    + pose helper_2b as H2. specialize (H2 t1 t2 t'). apply H2. apply H. 
-    + pose helper_2a as H2. specialize (H2 t1 t2 t'). apply H2. apply H. 
-Qed.
-
-
-
-(** 3.1 Declarations useful for the proof **)
-
-
-Axiom refl_comm :
-  forall t1 t2, t1 == t2 -> t2 == t1.
-
-Lemma subst_distr_opp :
-  forall s x y, apply_subst (x + y) s == apply_subst x s + apply_subst y s.
-Proof.
-  intros.
-  apply refl_comm.
-  apply subst_distribution.
-Qed. 
-
-
-Lemma subst_mul_distr_opp :
-  forall s x y, apply_subst (x * y) s == apply_subst x s * apply_subst y s.
-Proof.
-  intros.
-  apply refl_comm.
-  apply subst_associative.
-Qed. 
-
-
-Lemma sum_assoc_opp :
- forall x y z, x + (y + z) == (x + y) + z.
-Proof.
-Admitted.
-
-Lemma mul_assoc_opp :
- forall x y z, x * (y * z) == (x * y) * z.
-Proof.
-Admitted.
-
-
-Lemma var_subst:
-  forall (v : var) (ts : term) ,
-  (apply_subst (VAR v) (cons (v , ts) nil) ) == ts.
-Proof.
-Admitted.
-
-Lemma id_subst:
-  forall (t : term) (x : var),
-  apply_subst t [(x , VAR x)] == t.
-Proof.
-Admitted.
-
-   
-
-
-
-
-
-
-Definition sub_term (t : term) (t' : term) : Prop :=
-  forall (x : var ),
-  (In x (term_unique_vars t) ) -> (In x (term_unique_vars t')) .
-
-Lemma sub_term_v :
-  forall (v : var),
-  sub_term (VAR v) (VAR v).
- Proof.
-Admitted.
 
 Lemma sub_term_id :
   forall (t : term),
@@ -232,15 +39,12 @@ Lemma sub_term_id :
  Proof.
 Admitted.
 
-Fixpoint build_on_list_of_vars (list_var : var_set) (s : term) (sig1 : subst) (sig2 : subst) : subst :=
-  match list_var with 
-   | nil => nil 
-   | v' :: v =>
-      (cons (v' , (s + T1) * (apply_subst (VAR v') sig1 )  + s * (apply_subst (VAR v' ) sig2 )  )    
-            (build_on_list_of_vars v s sig1 sig2) )
-  end. 
 
 
+(* helper lemma: applying two different substitutions on the same variable give the same result. 
+    one subsitution containtains only replacement, and it is for this variable. The other subsitution
+    contains the previous replacement but also more replacements other variables (so the subsitution for 
+    the extra variables do not affect the application of the subsitution *)
 Lemma helper_1:
 forall (t' s : term) (v : var) (sig1 sig2 : subst),
   sub_term (VAR v) t' -> 
@@ -250,12 +54,17 @@ forall (t' s : term) (v : var) (sig1 sig2 : subst),
 Proof.
 Admitted.
 
+
+(* helper lemma : if the sum of two terms is a subterm of another term t', then each component of the sum is
+   also a subterm of the other term t' *)
 Lemma helper_2a:
   forall (t1 t2 t' : term),
   sub_term (t1 + t2) t' -> sub_term t1 t'.
 Proof.
 Admitted. 
   
+(* helper lemma : if the sum of two terms is a subterm of another term t', then each component of the sum is
+   also a subterm of the other term t' *)
 Lemma helper_2b:
   forall (t1 t2 t' : term),
   sub_term (t1 + t2) t' -> sub_term t2 t'.
@@ -264,9 +73,9 @@ Admitted.
 
 
 
+(** 3.3 Proof that Lownheim's algorithm unifes a given term **)
 
-
-(* Lemma 10.4.3*)
+(* Lemma 10.4.5*)
 
 Lemma subs_distr_vars_ver2 :
   forall (t t' : term) (s : term) (sig1 sig2 : subst),
@@ -292,7 +101,7 @@ Proof.
     + unfold term_unique_vars. unfold term_vars. unfold var_set_create_unique. unfold var_set_includes_var. unfold build_on_list_of_vars.
     rewrite var_subst. reflexivity. 
     + apply H. 
-  -  intros. specialize (IHt1 t'). specialize (IHt2 t').  repeat rewrite subst_distr_opp. 
+  -  intros. specialize (IHt1 t'). specialize (IHt2 t').  repeat rewrite subst_sum_distr_opp. 
       rewrite IHt1. rewrite IHt2.
     + rewrite distr. rewrite distr. repeat rewrite sum_assoc. rewrite sum_comm with (x := (s + T1) * apply_subst t2 sig1)
       (y := (s * apply_subst t1 sig2 + s * apply_subst t2 sig2)). repeat rewrite sum_assoc.
@@ -318,33 +127,102 @@ Proof.
     + pose helper_2a as H2. specialize (H2 t1 t2 t'). apply H2. apply H. 
 Qed.
 
+
+
+(* Utilizing lemma 10.4.5 with specific sigmas gives a substituion the unifies the term *)
 Lemma specific_sigmas_unify:
-  forall (t : term) (tau : subst) (x : var),
+  forall (t : term) (tau : subst),
   (unifier t tau) -> 
-  (apply_subst t (build_on_list_of_vars  (term_unique_vars t) t (cons (x , (VAR x)) nil ) tau )
+  (apply_subst t (build_on_list_of_vars  (term_unique_vars t) t (build_id_subst (term_unique_vars t)) tau )
   ) == T0 .
   Proof.
   intros. 
   rewrite subs_distr_vars_ver2.
-  + rewrite id_subst. rewrite mul_comm with (x := t + T1). rewrite distr. rewrite mul_x_x. rewrite mul_id_sym. rewrite sum_x_x.
+  - rewrite id_subst. rewrite mul_comm with (x := t + T1). rewrite distr. rewrite mul_x_x. rewrite mul_id_sym. rewrite sum_x_x.
     rewrite sum_id. 
     unfold unifier in H. rewrite H. rewrite mul_T0_x_sym. reflexivity.
-  +  apply sub_term_id.
+  -  apply sub_term_id.
 Qed.
 
-Definition eqv_lists {A : Type} (l1 : list A) (l2 : list A) : Prop :=
-forall (elt : A),
- In elt l1 <-> In elt l2.
-     
-Lemma specific_sigmas_is_lowengeim:
-forall (t : term) (tau : subst) (x : var),
- (unifier t tau) ->
-  eqv_lists
-(build_on_list_of_vars  (term_unique_vars t) t (cons (x , (VAR x)) nil ) tau )
-( lowenheim_subst t tau).
+(* Our lowenheim's subsitution builder unifies any given term *)
+Lemma lownheim_unifies:
+  forall (t : term) (tau : subst),
+  (unifier t tau) -> 
+  (apply_subst t (build_lowenheim_subst t tau)) == T0.
 Proof.
-intros. unfold eqv_lists. intros.
-split.
- - induction t.
-   + 
+intros. unfold build_lowenheim_subst. apply specific_sigmas_unify. apply H.
+Qed.
+
+
+
+
+
+(** 3.4 Proof that Lownheim's algorithm produces a reproductive unifier (mgu) **)
+
+
+(* definition of a reproductive unifier. We have a small modification than the book's, we are
+   defining a unifier to be reproductive for the all x in Var(t), not for all x in general ,
+  because our lownheim builder uses only variables from a term *)
+Definition reproductive_unifier (t : term) (sig : subst) : Prop :=
+  unifier t sig ->
+  forall (tau : subst) (x : var),
+  unifier t tau /\ (In x (term_unique_vars t))->
+  (apply_subst (apply_subst (VAR x) sig ) tau) == (apply_subst (VAR x) tau).
+
+
+(* converting identical terms boolean to Propositions *) 
+Lemma term_ident_prop :
+ forall (t1 t2 : term),
+  match identical t1 t2 with
+   | true => True
+   | false => False
+  end.
+ Proof. 
 Admitted.
+
+
+
+(* lemma: applying lowenheim's subtitution on the variable of a term gives us the initial format 
+  of the replacement for that variable (lowenheim's reverse application ) *)
+Lemma lowenheim_rephrase :
+  forall (t : term) (tau : subst) (x : var),
+  (unifier t tau) -> 
+  (In x (term_unique_vars t)) -> 
+  (apply_subst (VAR x) (build_lowenheim_subst t tau)) == 
+  (t + T1) * (VAR x) + t * (apply_subst (VAR x) tau).
+  Proof.
+intros. 
+induction t.
+  - unfold build_lowenheim_subst. unfold term_unique_vars. unfold term_vars. unfold var_set_create_unique.
+    unfold build_id_subst. unfold build_on_list_of_vars. rewrite mul_comm with (y := VAR x). rewrite distr.
+    rewrite mul_T0_x_sym. rewrite sum_id. rewrite mul_T0_x. rewrite mul_id_sym. rewrite sum_id_sym. unfold apply_subst. reflexivity.
+  - unfold term_unique_vars in H0. unfold term_vars in H0. unfold var_set_create_unique in H0. unfold In in H0. destruct H0.
+  - unfold build_lowenheim_subst. unfold term_unique_vars. unfold term_vars. unfold var_set_create_unique.
+    unfold var_set_includes_var. unfold term_unique_vars in H0. unfold term_vars in H0. unfold var_set_create_unique in H0. 
+    unfold var_set_includes_var in H0. unfold In in H0. simpl in H0.  destruct H0.
+    + rewrite H0. unfold build_id_subst. unfold build_on_list_of_vars. simpl. destruct beq_nat. 
+      {  reflexivity. }
+      { rewrite mul_comm with (y := VAR x). rewrite distr. rewrite mul_x_x. rewrite mul_id_sym. rewrite sum_x_x. rewrite sum_id.
+        rewrite H0 in H. unfold unifier in H. rewrite H. rewrite mul_T0_x_sym. pose proof term_ident_prop  as H1. specialize (H1 (VAR x) T0).
+        simpl in H1. destruct H1. }
+    +  destruct H0.
+  - 
+Admitted.
+
+
+
+(* lowenheim's algorithm gives a reproductive unifier, hence an mgu; because a reproductuve unifier is an mgu *)
+Lemma lowenheim_reproductive:
+  forall (t : term) (tau : subst),
+  (unifier t tau) -> 
+  reproductive_unifier t (build_lowenheim_subst t tau) .
+Proof.
+ intros. unfold reproductive_unifier. intros.   rewrite lowenheim_rephrase.
+  - rewrite subst_sum_distr_opp. rewrite subst_mul_distr_opp. rewrite subst_mul_distr_opp.
+    destruct H1. unfold unifier in H1. rewrite H1. rewrite mul_T0_x. rewrite subst_sum_distr_opp.
+    rewrite H1. rewrite ground_term_cannot_subst.
+    + rewrite sum_id. rewrite mul_id. rewrite sum_comm. rewrite sum_id. reflexivity.
+    + unfold ground_term. intuition.
+  - apply H.  
+  - destruct H1. apply H2.
+Qed.
